src3.0/Transforms/sas_msim.v
@@ -1,0 +1,495 @@
+Require Import Memory.
+Require Import Values.
+Require Import Coqlib.
+Require Import Integers.
+Require Import AST.
+Require Import Znumtheory.
+Require Import vellvm_tactics.
+Require Import memory_sim.
+
+Module SASmsim.
+
+(** * Generic injections *)
+
+(** A memory state [m1] generically injects into another memory state [m2] via the
+  memory injection [f] if the following conditions hold:
+- each access in [m2] that corresponds to a valid access in [m1]
+  is itself valid;
+- the memory value associated in [m1] to an accessible address
+  must inject into [m2]'s memory value at the corersponding address;
+- ignore data stored at [lo, hi) in block b, although they still need to be valid.
+*)
+
+Export Mem.
+
+Record mem_inj (f: meminj) (b:block) (lo hi:Z) (m1 m2: mem) : Prop :=
+  mk_mem_inj {
+    mi_access:
+      forall b1 b2 delta chunk ofs p,
+      f b1 = Some(b2, delta) ->
+      valid_access m1 chunk b1 ofs p ->
+      valid_access m2 chunk b2 (ofs + delta) p;
+    mi_memval:
+      forall b1 ofs b2 delta,
+      f b1 = Some(b2, delta) ->
+      perm m1 b1 ofs Nonempty ->
+      b1 <> b \/ (b1 = b /\ (ofs < lo \/ ofs >= hi)) ->
+      MoreMem.memval_inject f (m1.(mem_contents) b1 ofs) 
+        (m2.(mem_contents) b2 (ofs + delta))
+  }.
+
+(** Preservation of permissions *)
+
+Lemma perm_inj:
+  forall b lo hi f m1 m2 b1 ofs p b2 delta,
+  mem_inj f b lo hi m1 m2 ->
+  perm m1 b1 ofs p ->
+  f b1 = Some(b2, delta) ->
+  perm m2 b2 (ofs + delta) p.
+Proof.
+  intros. 
+  assert (valid_access m1 (Mint 7) b1 ofs p).
+    split. red; intros. simpl in H2. rewrite bytesize_chunk_7_eq_1 in H2. replace ofs0 with ofs by omega. auto.
+    simpl. apply Zone_divide.
+  exploit mi_access; eauto. intros [A B].
+  apply A. simpl; rewrite bytesize_chunk_7_eq_1; omega. 
+Qed.
+
+(** Preservation of loads. *)
+
+Lemma getN_inj:
+  forall b lo hi f m1 m2 b1 b2 delta,
+  mem_inj f b lo hi m1 m2 ->
+  f b1 = Some(b2, delta) ->
+  forall n ofs,
+  range_perm m1 b1 ofs (ofs + Z_of_nat n) Readable ->
+  b1 <> b \/ (b1 = b /\ (ofs + Z_of_nat n <= lo \/ ofs >= hi)) ->
+  list_forall2 (MoreMem.memval_inject f) 
+               (getN n ofs (m1.(mem_contents) b1))
+               (getN n (ofs + delta) (m2.(mem_contents) b2)).
+Proof.
+  induction n; intros; simpl.
+    constructor.
+
+    rewrite inj_S in *. 
+    constructor. 
+      eapply mi_memval; eauto.
+        apply perm_implies with Readable.
+          apply H1. omega. 
+          constructor. 
+        destruct H2 as [H2 | [H2 [H3 | H4]]]; subst; auto.
+        right. 
+        assert (J:=@Z_of_S_gt_O n).
+        split; try solve [auto | omega].
+
+      replace (ofs + delta + 1) with ((ofs + 1) + delta) by omega.
+      apply IHn. 
+        red; intros; apply H1; omega. 
+
+        destruct H2 as [H2 | [H2 [H3 | H4]]]; subst; try solve 
+          [auto | right; split; try solve [auto | omega]].
+Qed.
+
+Lemma load_inj:
+  forall b lo hi f m1 m2 chunk b1 ofs b2 delta v1,
+  MoreMem.meminj_no_overlap f ->
+  MoreMem.meminj_zero_delta f ->
+  mem_inj f b lo hi m1 m2 ->
+  load chunk m1 b1 ofs = Some v1 ->
+  f b1 = Some (b2, delta) ->
+  b1 <> b \/ (b1 = b /\ (ofs + size_chunk chunk <= lo \/ ofs >= hi)) ->
+  exists v2, 
+    load chunk m2 b2 (ofs + delta) = Some v2 /\ MoreMem.val_inject f v1 v2.
+Proof.
+Local Transparent load.
+  intros.
+  exists (decode_val chunk (getN (size_chunk_nat chunk) 
+            (ofs + delta) (m2.(mem_contents) b2))).
+  split. 
+    unfold load. apply pred_dec_true.  
+    eapply mi_access; eauto with mem. 
+
+    exploit load_result; eauto. intro. subst.
+    apply MoreMem.decode_val_inject; auto.
+    eapply getN_inj; eauto. 
+      rewrite <- size_chunk_conv. exploit load_valid_access; eauto. intros [A B]. auto.
+      rewrite <- size_chunk_conv. auto.
+Qed.
+
+(** Preservation of stores. *)
+
+Lemma setN_inj_inside:
+  forall delta f vl1 vl2,
+  list_forall2 (MoreMem.memval_inject f) vl1 vl2 ->
+  forall p c1 c2,
+  (forall q, p <= q < p + Z_of_nat (length vl1) ->
+             MoreMem.memval_inject f ((setN vl1 p c1) q) 
+                                     ((setN vl2 (p + delta) c2) (q + delta))).
+Proof.
+  induction 1; intros; simpl in *.
+    contradict H; omega.
+
+    replace (p + delta + 1) with ((p + 1) + delta) by omega.
+    destruct (Z_le_dec (p+1) q).
+      apply IHlist_forall2; auto. 
+      rewrite Zpos_P_of_succ_nat in H1.
+      auto with zarith.
+
+      assert (p = q) as EQ. omega. 
+      subst.
+      repeat rewrite setN_outside by omega.
+      rewrite update_s. rewrite update_s. auto.
+Qed.
+
+Lemma setN_inj_outside:
+  forall delta f vl1 vl2
+  (Heq: length vl1 = length vl2),
+  forall p c1 c2,
+  (forall q, MoreMem.memval_inject f (c1 q) (c2 (q + delta)) ->
+             p > q \/ q >= p + Z_of_nat (length vl1) ->
+             MoreMem.memval_inject f ((setN vl1 p c1) q) 
+                                     ((setN vl2 (p + delta) c2) (q + delta))).
+Proof.
+  intros.
+  repeat rewrite setN_outside by omega.
+  auto.
+Qed.
+
+(* go to Coqlib *)
+Lemma list_forall2_length_eq:
+  forall (A B: Type) (P1: A -> B -> Prop) (l1: list A) (l2: list B),
+  list_forall2 P1 l1 l2 -> length l1 = length l2.
+Proof.
+  induction 1; intros; auto.
+    simpl. congruence.
+Qed.
+
+Lemma store_mapped_inj:
+  forall b lo hi f chunk m1 b1 ofs v1 n1 m2 b2 delta v2,
+  mem_inj f b lo hi m1 m2 ->
+  store chunk m1 b1 ofs v1 = Some n1 ->
+  MoreMem.meminj_no_overlap f ->
+  f b1 = Some (b2, delta) ->
+  MoreMem.val_inject f v1 v2 ->
+  exists n2,
+    store chunk m2 b2 (ofs + delta) v2 = Some n2
+    /\ mem_inj f b lo hi n1 n2.
+Proof.
+  intros. inversion H. 
+  assert (valid_access m2 chunk b2 (ofs + delta) Writable).
+    eapply mi_access0; eauto with mem.
+  destruct (valid_access_store _ _ _ _ v2 H4) as [n2 STORE]. 
+  exists n2; split. eauto.
+  constructor.
+(* access *)
+  intros.
+  eapply store_valid_access_1; [apply STORE |].
+  eapply mi_access0; eauto.
+  eapply store_valid_access_2; [apply H0 |]. auto.
+(* mem_contents *)
+  intros.
+  assert (perm m1 b0 ofs0 Nonempty). eapply perm_store_2; eauto. 
+  rewrite (store_mem_contents _ _ _ _ _ _ H0).
+  rewrite (store_mem_contents _ _ _ _ _ _ STORE).
+  unfold update. 
+  destruct (zeq b0 b1). subst b0.
+  (* block = b1, block = b2 *)
+  assert (b3 = b2) by congruence. subst b3.
+  assert (delta0 = delta) by congruence. subst delta0.
+  rewrite zeq_true.
+  eapply mi_memval0 in H7; eauto.
+  apply MoreMem.encode_val_inject with (chunk:=chunk) in H3; auto.  
+  assert (length (encode_val chunk v1) = length (encode_val chunk v2)) as EQ.
+    eapply list_forall2_length_eq; eauto.
+  destruct (Z_gt_dec ofs ofs0).
+    apply setN_inj_outside; auto.
+    destruct (Z_ge_dec ofs0 (ofs + Z_of_nat (length (encode_val chunk v1)))).
+      apply setN_inj_outside; auto.
+      eapply setN_inj_inside; eauto. omega.
+
+  destruct (zeq b3 b2). subst b3.
+  (* block <> b1, block = b2 *)
+  rewrite setN_other. auto.
+  rewrite encode_val_length. rewrite <- size_chunk_conv. intros. 
+  assert (b2 <> b2).
+    eapply H1; eauto. 
+  congruence.
+  (* block <> b1, block <> b2 *)
+  eauto.
+Qed.
+
+Lemma store_mapped_inj_inside:
+  forall f chunk m1 b1 ofs v1 n1 m2 b2 delta v2,
+  mem_inj f b1 ofs (ofs+size_chunk chunk) m1 m2 ->
+  store chunk m1 b1 ofs v1 = Some n1 ->
+  MoreMem.meminj_no_overlap f ->
+  f b1 = Some (b2, delta) ->
+  MoreMem.val_inject f v1 v2 ->
+  exists n2,
+    store chunk m2 b2 (ofs + delta) v2 = Some n2
+    /\ MoreMem.mem_inj f n1 n2.
+Proof.
+  intros. inversion H. 
+  assert (valid_access m2 chunk b2 (ofs + delta) Writable).
+    eapply mi_access0; eauto with mem.
+  destruct (valid_access_store _ _ _ _ v2 H4) as [n2 STORE]. 
+  exists n2; split. eauto.
+  constructor.
+(* access *)
+  intros.
+  eapply store_valid_access_1; [apply STORE |].
+  eapply mi_access0; eauto.
+  eapply store_valid_access_2; [apply H0 |]. auto.
+(* mem_contents *)
+  intros.
+  assert (perm m1 b0 ofs0 Nonempty). eapply perm_store_2; eauto. 
+  rewrite (store_mem_contents _ _ _ _ _ _ H0).
+  rewrite (store_mem_contents _ _ _ _ _ _ STORE).
+  unfold update. 
+  destruct (zeq b0 b1). subst b0.
+  (* block = b1, block = b2 *)
+  assert (b3 = b2) by congruence. subst b3.
+  assert (delta0 = delta) by congruence. subst delta0.
+  rewrite zeq_true.
+  apply MoreMem.encode_val_inject with (chunk:=chunk) in H3; auto.  
+  assert (length (encode_val chunk v1) = length (encode_val chunk v2)) as EQ.
+    eapply list_forall2_length_eq; eauto.
+  destruct (Z_gt_dec ofs ofs0).
+    apply setN_inj_outside; auto.
+    eapply mi_memval0 in H7; eauto.
+      right. split; auto. omega.
+    destruct (Z_ge_dec ofs0 (ofs + Z_of_nat (length (encode_val chunk v1)))).
+      apply setN_inj_outside; auto.
+      eapply mi_memval0 in H7; eauto.
+        rewrite encode_val_length in z. rewrite <- size_chunk_conv in z.
+        right. split; auto.
+
+      eapply setN_inj_inside; eauto. omega.
+
+  destruct (zeq b3 b2). subst b3.
+  (* block <> b1, block = b2 *)
+  rewrite setN_other. auto.
+  rewrite encode_val_length. rewrite <- size_chunk_conv. intros. 
+  assert (b2 <> b2).
+    eapply H1; eauto. 
+  congruence.
+  (* block <> b1, block <> b2 *)
+  eauto.
+Qed.
+
+Lemma store_unmapped_inj:
+  forall b lo hi f chunk m1 b1 ofs v1 n1 m2,
+  mem_inj f b lo hi m1 m2 ->
+  store chunk m1 b1 ofs v1 = Some n1 ->
+  f b1 = None ->
+  mem_inj f b lo hi n1 m2.
+Proof.
+  intros. inversion H.
+  constructor.
+(* access *)
+  eauto with mem.
+(* mem_contents *)
+  intros. 
+  rewrite (store_mem_contents _ _ _ _ _ _ H0).
+  rewrite update_o. eauto with mem. 
+  congruence.
+Qed.
+
+Lemma store_outside_inj:
+  forall b0 lo0 hi0 f m1 m2 chunk b ofs v m2',
+  mem_inj f b0 lo0 hi0 m1 m2 ->
+  (forall b' delta ofs',
+    f b' = Some(b, delta) ->
+    perm m1 b' ofs' Nonempty ->
+    ofs' + delta < ofs \/ ofs' + delta >= ofs + size_chunk chunk) ->
+  store chunk m2 b ofs v = Some m2' ->
+  mem_inj f b0 lo0 hi0 m1 m2'.
+Proof.
+  intros. inversion H. constructor.
+(* access *)
+  eauto with mem.
+(* mem_contents *)
+  intros. 
+  rewrite (store_mem_contents _ _ _ _ _ _ H1).
+  unfold update. destruct (zeq b2 b). subst b2.
+  rewrite setN_outside. auto. 
+  rewrite encode_val_length. rewrite <- size_chunk_conv. 
+  eapply H0; eauto. 
+  eauto with mem.
+Qed.
+
+(** Preservation of allocations *)
+
+Lemma alloc_right_inj:
+  forall b9 lo9 hi9 f m1 m2 lo hi b2 m2',
+  mem_inj f b9 lo9 hi9 m1 m2 ->
+  alloc m2 lo hi = (m2', b2) ->
+  mem_inj f b9 lo9 hi9 m1 m2'.
+Proof.
+  intros. injection H0. intros NEXT MEM.
+  inversion H. constructor.
+(* access *)
+  intros. eauto with mem. 
+(* mem_contents *)
+  intros.
+  assert (valid_access m2 (Mint 7) b0 (ofs + delta) Nonempty).
+    eapply mi_access0; eauto.
+    split. 
+      simpl. red; intros. 
+      rewrite bytesize_chunk_7_eq_1 in H4. 
+      assert (ofs0 = ofs) by omega. congruence.
+
+      simpl. apply Zone_divide. 
+  assert (valid_block m2 b0) by eauto with mem.
+Local Transparent alloc.
+  rewrite <- MEM; simpl. 
+  rewrite update_o. 
+    eauto with mem.
+    unfold valid_block in H5. omega.
+Qed.
+
+Lemma alloc_left_unmapped_inj:
+  forall b9 lo9 hi9 f m1 m2 lo hi m1' b1,
+  mem_inj f b9 lo9 hi9 m1 m2 ->
+  alloc m1 lo hi = (m1', b1) ->
+  f b1 = None ->
+  mem_inj f b9 lo9 hi9 m1' m2.
+Proof.
+  intros. inversion H. constructor.
+(* access *)
+  unfold update; intros.
+  exploit valid_access_alloc_inv; eauto. unfold eq_block. intros. 
+  destruct (zeq b0 b1). congruence. eauto.
+(* mem_contents *)
+  injection H0; intros NEXT MEM. intros. 
+  rewrite <- MEM; simpl. rewrite NEXT. unfold update.
+  exploit perm_alloc_inv; eauto. intros. 
+  destruct (zeq b0 b1). 
+    subst. congruence.
+    eauto.
+Qed.
+
+Lemma free_right_inj:
+  forall b9 lo9 hi9 f m1 m2 b lo hi m2',
+  mem_inj f b9 lo9 hi9 m1 m2 ->
+  free m2 b lo hi = Some m2' ->
+  (forall b1 delta ofs p,
+    f b1 = Some(b, delta) -> perm m1 b1 ofs p ->
+    lo <= ofs + delta < hi -> False) ->
+  mem_inj f b9 lo9 hi9 m1 m2'.
+Proof.
+  intros. exploit free_result; eauto. intro FREE. inversion H. constructor.
+(* access *)
+  intros. exploit mi_access0; eauto. intros [RG AL]. split; auto.
+  red; intros. eapply perm_free_1; eauto. 
+  destruct (zeq b2 b); auto. subst b. right.
+  destruct (zlt ofs0 lo); auto. destruct (zle hi ofs0); auto.
+  elimtype False. eapply H1 with (ofs := ofs0 - delta). eauto. 
+  apply H3. omega. omega.
+(* mem_contents *)
+  intros. rewrite FREE; simpl.
+  specialize (mi_memval0 _ _ _ _ H2 H3).
+  assert (b=b2 /\ lo <= ofs+delta < hi \/ 
+          (b<>b2 \/ ofs+delta<lo \/ hi <= ofs+delta)) as J 
+    by (unfold block; omega).
+  destruct J as [[J1 J2] | J]; subst.
+    specialize (H1 _ _ _ _ H2 H3). elimtype False; auto.
+    rewrite (clearN_out _ _ _ _ _ _ J); auto.
+Qed.
+
+Lemma free_inj:
+  forall b9 lo9 hi9 f m1 m2 b1 b2 delta lo hi m1' m2',
+  MoreMem.meminj_no_overlap f ->
+  MoreMem.meminj_zero_delta f ->
+  mem_inj f b9 lo9 hi9 m1 m2 ->
+  free m1 b1 lo hi = Some m1' ->
+  free m2 b2 (lo+delta) (hi+delta) = Some m2' ->
+  f b1 = Some (b2, delta) ->
+  mem_inj f b9 lo9 hi9 m1' m2'.
+Proof.
+  intros b9 lo9 hi9 f m1 m2 b1 b2 delta lo hi m1' m2' J J' H H0 H1 H2.
+  exploit free_result; eauto. 
+  intro FREE. inversion H. constructor.
+(* access *)
+  intros. exploit mi_access0; eauto with mem. 
+  intros [RG AL]. split; auto.
+  red; intros. eapply perm_free_1; eauto. 
+  destruct (zeq b3 b2); auto. 
+    subst b2. right.
+    destruct (zlt ofs0 (lo + delta)); auto. 
+    destruct (zle (hi + delta) ofs0); auto.
+    destruct (@MoreMem.meminj_no_overlap_spec f b0 b3 delta0 b1 delta J H3 H2)
+      as [G1 G2]; subst.
+    assert (lo <= ofs0 - delta < hi) as J1.
+      clear - z z0. auto with zarith.
+    assert (ofs <= ofs0 - delta < ofs + size_chunk chunk) as J2.
+      clear - H5. auto with zarith.
+    destruct H4 as [H41 H42].
+    apply H41 in J2.
+    eapply perm_free_2 with (p:=p) in J1; eauto.
+    congruence.
+(* mem_contents *)
+  intros. rewrite FREE; simpl.
+  assert (FREE':=H0). apply free_result in FREE'.
+  rewrite FREE'; simpl.   
+  assert (b0=b1 /\ lo <= ofs < hi \/ (b1<>b0 \/ ofs<lo \/ hi <= ofs)) as J1
+    by (unfold block; omega).
+  assert (b2=b3 /\ lo+delta <= ofs+delta < hi+delta \/ 
+    (b2<>b3 \/ ofs+delta<lo+delta \/ hi+delta <= ofs+delta)) 
+    as J2 by (unfold block; omega).
+  destruct J1 as [J1 | J1].
+    destruct J1 as [J11 J12]; subst.
+    eapply perm_free_2 with (p:=Nonempty) in H0; eauto.
+    congruence.
+
+    rewrite (clearN_out _ _ _ _ _ _ J1).
+    destruct J2 as [J2 | J2].
+      destruct J2 as [J21 J22]; subst.
+      destruct (@MoreMem.meminj_no_overlap_spec f b0 b3 delta0 b1 delta J H3 H2)
+        as [G1 G2]; subst.
+      assert (lo <= ofs < hi) as EQ.
+        clear - J22. auto with zarith.
+      clear - J1 EQ.
+      destruct J1 as [J1 | J1]; try solve [congruence].
+      contradict EQ; auto with zarith.
+
+      assert (W1:=H2). apply J' in W1. subst.
+      assert (W2:=H3). apply J' in W2. subst.
+      rewrite (clearN_out _ _ _ _ _ _ J2).
+      eapply perm_free_3 in H4; eauto.
+Qed.
+
+Lemma free_left_nonmap_inj:
+  forall b9 lo9 hi9 f m1 m2 b lo hi m1' (Hprop: f b = None),
+  mem_inj f b9 lo9 hi9 m1 m2 ->
+  Mem.free m1 b lo hi = Some m1' ->
+  mem_inj f b9 lo9 hi9 m1' m2.
+Proof.
+  intros. exploit Mem.free_result; eauto. intro FREE. inversion H. constructor.
+(* access *)
+  intros. eauto with mem.
+(* mem_contents *)
+  intros. rewrite FREE; simpl.
+  assert (b=b1 /\ lo <= ofs < hi \/ (b<>b1 \/ ofs<lo \/ hi <= ofs)) as J
+    by (unfold Values.block; omega).
+  destruct J as [[J1 J2] | J]; subst.
+    uniq_result.
+
+    rewrite (Mem.clearN_out _ _ _ _ _ _ J).
+    apply mi_memval0; auto.
+    eapply Mem.perm_free_3; eauto.
+Qed.
+
+Lemma inject_id_no_overlap: MoreMem.meminj_no_overlap inject_id.
+Proof.
+  unfold MoreMem.meminj_no_overlap, inject_id.
+  intros. uniq_result. auto.
+Qed.
+
+Lemma inject_id_zero_delta: MoreMem.meminj_zero_delta inject_id.
+Proof.
+  unfold MoreMem.meminj_zero_delta, inject_id.
+  intros. uniq_result. auto.
+Qed.
+
+End SASmsim.
